coq/coq/Translation.v
@@ -1,0 +1,66 @@
+Require Import LibTactics.
+Require Import Metalib.Metatheory.
+Require Import List. Import ListNotations.
+Require Import Arith Lia.
+Require Import Strings.String.
+Require Import Sorting.Permutation.
+Require Import Sorting.Sorted.
+Require Export Infrastructure.
+
+
+Reserved Notation "|[ A ]|" (at level 5, A at next level).
+
+Fixpoint styp2ttyp (A: typ) : ttyp := ttyp_base
+where "|[ A ]|" := (styp2ttyp A).
+
+Notation "|| A ||" := (type2index A) (at level 1, A at next level). (* too high *)
+
+(* Properties of translation (to type index) functions *)
+(* Lemma tindex_trans_arrow : forall A B, *)
+(*     || (typ_arrow A B) || = ti_arrow || B ||. *)
+(* Admitted. *)
+(* Lemma tindex_trans_rcd : forall l A, *)
+(*     || (typ_rcd l A) || = ti_rcd l || A ||. *)
+(* Admitted. *)
+
+(* Properties of translation (to target type) functions *)
+
+Lemma ttyp_trans_wf : forall A,
+    wf_typ |[A]|.
+Admitted.
+
+(* Typ-TopAbs requires no ord *)
+Lemma ttyp_trans_ord_top : forall A,
+    toplike A -> |[A]| = ttyp_top.
+Admitted.
+
+Lemma ttyp_trans_ord_ntop : forall A,
+    ord A -> ~ toplike A -> exists B, |[A]| = ttyp_rcd ||A|| B ttyp_top /\ wf_typ B.
+Admitted.
+
+Lemma ttyp_trans_base :
+    |[typ_base]| = ttyp_rcd ||typ_base|| ttyp_base ttyp_top.
+Admitted.
+
+Lemma ttyp_trans_ord_ntop_arrow : forall A A',
+    (* ord A -> ~ toplike A -> *) (* S-arrow requires no precondition *)
+    |[(typ_arrow A' A)]| = ttyp_rcd (ti_arrow || A ||) (ttyp_arrow |[A']| |[A]|) ttyp_top.
+Admitted.
+
+Lemma ttyp_trans_rcd : forall l A,
+    (* ord A -> ~ toplike A -> *) (* S-arrow requires no precondition *)
+    |[(typ_rcd l A)]| = ttyp_rcd (ti_rcd l || A ||) |[A]| ttyp_top.
+Admitted.
+
+Lemma ttyp_trans_and : forall A B C,
+    concat_typ |[ A ]| |[ B ]| C -> |[ (typ_and A B) ]| = C.
+Admitted.
+
+(* Properties about type translation *)
+Lemma concat_source_intersection : forall A B,
+    concat_typ |[ A ]| |[ B ]| |[ (typ_and A B) ]|.
+Admitted.
+
+Lemma translate_to_record_types : forall A,
+    rec_typ |[ A ]|.
+Admitted.
