coq/coq/TypeSafety.v
@@ -5,110 +5,17 @@ Require Import Arith Lia.
 Require Import Strings.String.
 Require Import Sorting.Permutation.
 Require Import Sorting.Sorted.
-Require Export Infrastructure.
+Require Export Translation.
+Require Export Target.
 (* Require Export Source3. *)
 
-
-Reserved Notation "|[ A ]|" (at level 5, A at next level).
-
-Fixpoint styp2ttyp (A: typ) : ttyp := ttyp_base
-where "|[ A ]|" := (styp2ttyp A).
-
-Notation "|| A ||" := (type2index A) (at level 1, A at next level). (* too high *)
-
-(* Properties of translation (to type index) functions *)
-Lemma tindex_trans_arrow : forall A B,
-    || (typ_arrow A B) || = ti_arrow || B ||.
-Admitted.
-Lemma tindex_trans_rcd : forall l A,
-    || (typ_rcd l A) || = ti_rcd l || A ||.
-Admitted.
-
-(* Properties of translation (to target type) functions *)
-
-Lemma ttyp_trans_wf : forall A,
-    wf_typ |[A]|.
-Admitted.
-
-(* Typ-TopAbs requires no ord *)
-Lemma ttyp_trans_ord_top : forall A,
-    toplike A -> |[A]| = ttyp_top.
-Admitted.
-
-Lemma ttyp_trans_ord_ntop : forall A,
-    ord A -> ~ toplike A -> exists B, |[A]| = ttyp_rcd ||A|| B ttyp_top /\ wf_typ B.
-Admitted.
-
-Lemma ttyp_trans_base :
-    |[typ_base]| = ttyp_rcd ||typ_base|| ttyp_base ttyp_top.
-Admitted.
-
-Lemma ttyp_trans_ord_ntop_arrow : forall A A',
-    (* ord A -> ~ toplike A -> *) (* S-arrow requires no precondition *)
-    |[(typ_arrow A' A)]| = ttyp_rcd (ti_arrow || A ||) (ttyp_arrow |[A']| |[A]|) ttyp_top.
-Admitted.
-
-Lemma ttyp_trans_rcd : forall l A,
-    (* ord A -> ~ toplike A -> *) (* S-arrow requires no precondition *)
-    |[(typ_rcd l A)]| = ttyp_rcd (ti_rcd l || A ||) |[A]| ttyp_top.
-Admitted.
-
-Lemma ttyp_trans_and : forall A B C,
-    concat_typ |[ A ]| |[ B ]| C -> |[ (typ_and A B) ]| = C.
-Admitted.
-
-(* Standard properties of typing *)
-
-Lemma target_typing_wf : forall E t A,
-    target_typing E t A -> uniq E.
-Proof with eauto; destruct_uniq; solve_uniq.
-  introv H.
-  induction* H.
-  - pick_fresh x. forwards*: H1 x...
-  - pick_fresh x. forwards*: H0 x...
-Qed.
-
-
-(* proved in TG *)
-Lemma target_weakening_simpl : forall E F e T,
-    target_typing E e T ->
-    uniq (F ++ E) ->
-    target_typing (F ++ E) e T.
-Admitted.
-
-(* Auxiliary tactics *)
-
-Lemma spl_decrease_size: forall A B C,
-    spl A B C -> size_typ B < size_typ A /\ size_typ C < size_typ A.
-Proof with (pose proof (size_typ_min_mutual); simpl in *; try lia).
-  introv H.
-  induction H; simpl in *; eauto...
-Qed.
-
-Ltac spl_size :=
-  try repeat match goal with
-         | [ H: spl _ _ _ |- _ ] =>
-           ( lets (?&?): spl_decrease_size H; clear H)
-    end.
-
-Ltac elia :=
-  try solve [pose proof (size_typ_min_mutual);
-             spl_size; simpl in *; try lia].
-
-Ltac indTypSize s :=
-  assert (SizeInd: exists i, s < i) by eauto;
-  destruct SizeInd as [i SizeInd];
-  repeat match goal with | [ h : typ |- _ ] => (gen h) end;
-  induction i as [|i IH]; [
-    intros; match goal with | [ H : _ < 0 |- _ ] => inverts H end
-  | intros ].
 
 (* Type safety *)
 (** The key is to prove the lookup label does exists in the record *)
 (** To prove type safety, we need to translate typing contexts / types
  \ x : A . e : B  => A->B ~> \ x . |e| ??? **)
 
-#[local] Hint Resolve target_typing_wf ttyp_trans_wf : core.
+#[local] Hint Resolve target_typing_wf_1 target_typing_wf_2 ttyp_trans_wf : core.
 #[local] Hint Unfold Tlookup : core.
 
 (* Definition subtype_wrt_lookup A B := *)
@@ -171,40 +78,87 @@ Ltac indTypSize s :=
 
 Lemma target_flex_typing_wf : forall E t A,
     target_flex_typing E t A -> uniq E.
-Proof with eauto using target_typing_wf; destruct_uniq; solve_uniq.
+Proof with eauto using target_typing_wf_1; destruct_uniq; solve_uniq.
   introv H.
   induction* H.
 Qed.
 
 #[local] Hint Resolve target_flex_typing_wf : core.
 
+#[local] Hint Constructors target_typing : core.
+
+(** flex_typing relaxes target typing **)
 Lemma flex_typing_property0 : forall E t A,
-    target_typing E t |[A]| ->
-    target_flex_typing E t |[A]|.
-Admitted.
+    target_typing E t |[A]| -> target_flex_typing E t |[A]|.
+Proof.
+  introv H.
+  applys* TFTyping_Orig.
+Qed.
+
+
+(** every lookup can be separately typed **)
+Lemma flex_typing_property3 : forall E t At ll Ct,
+    target_flex_typing E t At -> Tlookup ll At = Some Ct ->
+    exists Bt, target_typing E t Bt /\ Tlookup ll Bt = Some Ct.
+Proof.
+  introv HT HL. gen ll Ct.
+  induction HT; intros.
+  - eauto.
+  - solve_by_invert.
+  - inverts HL. case_if. exists* At.
+    inverts H2. subst*.
+  - inverts HL. case_if.
+    + inverts H0. subst.
+      forwards*: IHHT1 ll Ct. case_if*.
+    + forwards (?&?&?): IHHT2 H0.
+      exists* x. rewrite* H0.
+  - exists* At.
+    forwards (?&?&?): IHHT l At. case_if*.
+    eauto.
+Qed.
+
+(** flex_typing on well-typed terms only **)
+Lemma flex_typing_wt : forall E t A,
+    target_flex_typing E t A -> exists B, target_typing E t B.
+Proof.
+  introv HT. induction* HT.
+  - forwards* (?&?&?): flex_typing_property3 l At HT.
+    simpl. case_if*.
+Qed.
+
+
+(** top is the supertype in flex_typing  **)
+Lemma flex_typing_top : forall E t A,
+    target_flex_typing E t A -> target_flex_typing E t ttyp_top.
+Proof.
+  introv H. forwards*: flex_typing_wt H.
+Qed.
+
 
 Lemma flex_typing_property1 : forall E t A B,
     target_flex_typing E t |[typ_and A B]| ->
     target_flex_typing E t |[A]| /\ target_flex_typing E t |[B]|.
-Admitted.
+Proof with eauto using flex_typing_top.
+  introv H.
+  lets HC: concat_source_intersection A B.
+  inductions HC...
+  - split.
+    + rewrite <- x0...
+    + rewrite x...
+Qed.
 
-(* non-deterministic lookup works *)
-Lemma flex_typing_property2 : forall E t At Bt ll,
-    target_flex_typing E t At -> contained_by_rec_typ At ll Bt ->
-    target_typing E (texp_proj t ll) Bt.
-Admitted.
+(* (* non-deterministic lookup works *) *)
+(* Lemma flex_typing_property2 : forall E t At Bt ll, *)
+(*     target_flex_typing E t At -> contained_by_rec_typ At ll Bt -> *)
+(*     target_typing E (texp_proj t ll) Bt. *)
+(* Admitted. *)
 
-(* every lookup can be separately typed *)
-Lemma flex_typing_property3 : forall E t At ll Ct,
-    target_flex_typing E t At -> Tlookup ll At = Some Ct ->
-    exists Bt, target_typing E t Bt /\ Tlookup ll Bt = Some Ct.
-Admitted.
 
-(* every non-deterministic lookup can be separately typed *)
-Lemma flex_typing_property3_alter : forall E t At ll Ct,
-    target_flex_typing E t At -> contained_by_rec_typ At ll Ct ->
-    exists Bt, target_typing E t Bt /\ Tlookup ll Bt = Some Ct.
-Admitted.
+(* (* every non-deterministic lookup can be separately typed *) *)
+(* Lemma flex_typing_property3_alter : forall E t At ll Ct, *)
+(*     target_flex_typing E t At -> contained_by_rec_typ At ll Ct -> *)
+(*     exists Bt, target_typing E t Bt /\ Tlookup ll Bt = Some Ct. *)
+(* Admitted. *)
 
 Lemma comerge_split : forall t1 A1 t B t2 A2,
     comerge t1 A1 B t2 A2 t -> spl B A1 A2.
@@ -215,14 +169,6 @@ Proof.
     pick fresh x. applys* H0.
 Qed.
 
-(* Properties about type translation *)
-Lemma concat_source_intersection : forall A B,
-    concat_typ |[ A ]| |[ B ]| |[ (typ_and A B) ]|.
-Admitted.
-
-Lemma translate_to_record_types : forall A,
-    rec_typ |[ A ]|.
-Admitted.
 
 (* new property: same label means same type *)
 Lemma comerge_well_typed : forall E t1 A1 t B t2 A2,
@@ -239,7 +185,7 @@ Proof with elia; eauto.
     applys* TTyping_RcdCons.
     pick fresh x and apply TTyping_Abs...
     forwards* Hc: H x.
-    forwards: IH ((x, |[ A ]|) :: E) Hc...
+    forwards: IH ( ( x, |[ A ]| ) :: E) Hc...
     1-2: applys TTyping_App...
     1-2: applys TTyping_RcdProj...
     1,3: rewrite_env ( [ (x, |[ A ]|) ] ++  E); applys target_weakening_simpl.
@@ -399,7 +345,7 @@ Lemma distapp_well_typed_app : forall A B C G t1 t2 t3,
     appdist A (typ_arrow B C) -> target_flex_typing ||[ G ]|| t1 |[A]| ->
     target_flex_typing ||[ G ]|| t2 |[B]| -> distapp t1 A (tvl_exp t2) t3 ->
     target_typing ||[ G ]|| t3 |[C]|.
-Proof with eauto using target_typing_wf.
+Proof with eauto using target_typing_wf_1.
   introv HA HTa HTb HD. gen t1 t2.
   inductions HA; intros; inverts HD...
   - rewrite* ttyp_trans_ord_top.
@@ -421,7 +367,7 @@ Lemma distapp_well_typed_proj : forall A l B G t1 t3,
     appdist A (typ_rcd l B) -> target_typing ||[ G ]|| t1 |[A]| ->
     distapp t1 A (tvl_la l) t3 ->
     target_typing ||[ G ]|| t3 |[B]|.
-Proof with eauto using target_typing_wf.
+Proof with eauto using target_typing_wf_1.
   introv HA HT HD.
   inductions HA; inverts HD...
   - rewrite ttyp_trans_rcd in HT...
@@ -433,7 +379,7 @@ Qed.
 Theorem elaboration_well_typed : forall G e dirflag A t,
     elaboration G e dirflag A t ->
     target_typing ||[ G ]|| t |[A]|.
-Proof with eauto using translate_to_record_types, target_typing_wf, ctx_trans_preserves_uniq.
+Proof with eauto using translate_to_record_types, target_typing_wf_1, ctx_trans_preserves_uniq.
   introv HT.
   induction HT...
   - rewrite* ttyp_trans_ord_top.
